Update BB_denotations

BB_denotations.v
@@ -116,25 +116,44 @@ Definition BJump_sem (BB_end: BDenote) (jmp_dist1: nat) (jmp_dist2: option nat) 
 (* Should move the Theorem elsewhere, but it just came to me that we need it *)
 Fixpoint is_seq_cmds (cmds : list cmd) : bool :=
   match cmds with
-
   | CAsgn x e :: tl => is_seq_cmds tl
-
   | CIf e c1 c2 :: tl => false
-
   | CWhile pre e body :: tl => false
-
   | _ => true
 
   end.
 
-(* TODO: the cmds in the BBs generated are all BAsgn. *)
 
-(*  *)
-(* Fixpoint BAsgn_list_sem (BAsgn_sem_list: list BB_state) : BB_state :=
-  match BAsgn_sem_list with 
-  | cmd :: tl => BAsgn_sem ∘ BAsgn_list_sem tl
+Fixpoint BB_list_only_asgn (BBs: list BasicBlock): bool :=
+  match BBs with
+  | BB :: tl => 
+    if (is_seq_cmds BB.(cmd)) then 
+      BB_list_only_asgn tl
+    else
+      false
+  | _ => true
+  end.
+
+
+(* TODO: the cmds in the BBs generated are all BAsgn. *)
+Theorem BB_cmds_only_asgn:
+  forall cmds,
+    BB_list_only_asgn (BB_gen cmds) = true.
+Proof.
+  Admitted.
+
+
+  (* ! Flawed *)
+Fixpoint BAsgn_list_sem (BAsgn_sem_list: list BDenote) : BDenote := {|
+  nrm := match BAsgn_sem_list with 
+  | cmd :: tl => BAsgn_sem.(nrm) ∘ (BAsgn_list_sem tl).(nrm)
   | _ => Rels.id × Rels.id
-  end. *)
+  end;
+  err := ∅;
+  inf := ∅;
+|}.
+  
+    
 
 
 (* Combine list of BAsgn and the final BJump *)
